---
aliases: [3-body problem, the three body problem, three body problem, TBP, RTBP]
subject: Numerical Methods for Dynamical Systems
lecturer: Mercè Ollé Torner
format: in-person
program: Master in Advanced Mathematics and Mathematical Engineering
dates: 18-10-2022, 25-10-2022
tags: #mamme #numericalmethods #dynamicalsystems
---
## The restricted three-body problem (RTBP)
*Ref*: V. Szebehely, "Theory of orbits"

Assume 2 points bodies, called primaries, $P_1$, $P_2$, with masses $m_{1}\leq m_{2}$, that describe circular orbits arround their common center of mass located at the origin on the plan ($X, Y$) -- [sidereal](https://en.wikipedia.org/wiki/Sidereal_time) or nonrotating coordinates.

Assume a third body $P_3$, with infinitessimal mass, $m_{3}\approx 0$ such that $m_{1}$ and $m_2$ have influence (gravitational force) on $P_3$, but $P_3$ does not influence the motion of $P_{1}$ and $P_{2}$. 

$$\begin{cases}
\vec{R}_{1}(t^{*}) &= (X_{1}(t^{*}), Y_{1}(t^{*})) = (b\cos{(nt^{*})}, b\sin{(nt^{*})})  \\
\vec{R}_{2}(t^{*}) &= (X_{2}(t^{*}), Y_{2}(t^{*})) = (-a\cos{(nt^{*})}, -a\sin{(nt^{*})}) 
\end{cases}$$
Now, I'd like to know the motion of $P_{3}$.
![[3-body_problem_ini_diagram]]

By the Newton's law:

$$m_{3}\ddot{\vec{R}} = - G \frac{m_{3}m_{1}(\vec{R}-\vec{R}_1)}{||\vec{R} - \vec{R}_{1}||^{3}} - G\frac{m_{3}m_{2}(\vec{R}-\vec{R}_2)}{||\vec{R} - \vec{R}_{2}||^{3}}  = $$
where the dot notation is the derivative with respect to time ($t^*$).

This is a system of 2 ODE of 2nd order or ,equivalently, a system of 4 ODE of 1st order, non-autonomous (it depends on $t^{*}$).

Now let us consider a new system of coordinates $(x, y)$ -- synodical or rotating -- such that the primaries remain fixed on the x axis.

$$\begin{pmatrix}X \\ Y\end{pmatrix} = \begin{pmatrix}\cos{nt^{*}}  & -\sin{nt^{*}}  \\ \sin{nt^{*}}  & \cos{nt^{*}}\end{pmatrix}$$

or $$\begin{pmatrix}x \\ y \end{pmatrix} = \begin{pmatrix}\cos{nt^{*}}  & \sin{nt^{*}}  \\ - \sin{nt^{*}}  & \cos{nt^{*}}\end{pmatrix}\begin{pmatrix}X \\ Y\end{pmatrix}$$
Now we choose suitable units of mass, length and time such that $n=1$, $a+b=1$, $G=1$, $m_{1}+ m_{2}= 1$ (see *V.S*). Denote $t$ this new time.

$$\begin{cases}
x'' - 2y' &= \frac{\partial\Omega}{\partial x} \\
y'' + 2x' &= \frac{\partial\Omega}{\partial y}
\end{cases}$$
where $^{'} = \frac{d}{dt}$, $\Omega(x,y) = \frac{1}{2}(x^{2}+y^{2}) + \frac{1-\mu}{r_{1}} + \frac{\mu}{r_{2}} + \frac{1}{2}\mu(1-\mu)$
where $\mu = \frac{m_{2}}{m_{1}+m_{2}} \in (0, 0.5]$ , $r_{1}=dist(P_{1}, P_{3})$, $r_{2}=dist(P_{2}, P_{3}))$.
![[3_body_problem_rotating_frame]]
Then,
###### Def | Position vectors
$$\begin{cases}
r_{1} &= \sqrt{(x-\mu)^{2} + y^{2}} \\
r_{2} &= \sqrt{(x-\mu + 1)^{2} + y^{2}}
\end{cases}$$

This system is now autonomous. 

##### Exercise 1
Check that this expression
$$ 2 \Omega(x, y) - (x'^{2} + y'^{2}) = C$$
is a first integral called **[[Jacobi first integral]]**

##### Exercise 2
**2.1.** The system of ODE can be written as a Hamiltonian System with 2 degrees of freedom. taking
$x_{1}=x$, $x_{2}=y$, $y_{1}=x'-y$, $y_{2}= y' + x$
and Hamiltonian function
$$H(x_{1}, x_{2}, y_{1}, y_{2}) = \frac{1}{2}(y_{1}^{2}+y_{2}^{2}) +x_{2}y_{1}-x_{1}y_{2} - \left(\frac{1-\mu}{r_{1}} + \frac{\mu}{r_{2}}\right)$$
![[2.1. The 3 body problem 2022-11-14 18.14.30.excalidraw]]
The Hamiltonian system of ODE is
$$\begin{cases}
x_{i}' &= \frac{dx_{i}}{dt}=\frac{\partial H}{\partial y_i} \\
y_{i}' &= \frac{dy_{i}}{dt}=-\frac{\partial H}{\partial x_i}
\end{cases}$$

Recall that, in general, given a Hamiltonian function with $n$ degrees of freedom, $H(x_{1}, \dots, x_{n}, y_{1}, \dots, y_{n})$, the associated Hamiltonian system of ODE is
$$\begin{cases}
x_{i}' &= \frac{dx_{i}}{dt}=\frac{\partial H}{\partial y_i} \\
y_{i}' &= \frac{dy_{i}}{dt}=-\frac{\partial H}{\partial x_i}
\end{cases} \qquad i = 1,\dots, n$$
**2.2** Prove that $H(x,y) =H(x_{1}, \dots, x_{n}, y_{1}, \dots, y_{n})$ is a first integral for the Hamiltonian System. 
> This is just one line. dH/dt?

**2.3** Write the relation between $H = h$ and $C$ (the relation can only contain $h$, $C$, $\mu$).

For short, we can also write it like
$$\begin{cases}
x'' - 2y' &= \Omega_x \\
y'' + 2x' &= \Omega_y
\end{cases}$$
**Comments**: 
> Why do we add the term  $\frac{1}{2}\mu(1-\mu)$ for $\Omega$ if it doesn't play a role in the ODE? Just because you want $\Omega$ to take easy numbers for specific values of x, y

1. A first generalization of the RTBP is to consider the spatial RTBP, that is, $P_1$ and $P_2$ are fixed on the $x$ axis (they move on the ($X, Y$) system), but $P_3$ moves  in $(x, y, z)$ (or $(X, Y, Z)$). We obtain a system of 6 ODE of first order. 
2. A second generalization has to do with the 2-body motion of the primaries $P_{1}, P_{2}$:
	- Circular orbits -> *Circular RTBP*
	- Elliptic orbits -> *Elliptic RTBP*
	- Parabolic orbits -> *Parabolic RTBP*
	- Hyperbolic orbits -> *Hyperbolic RTBP*
3. The RTBP can be (has been) used as a preliminary model to explain:
	- Several real missions: Genesis, Artemis, etc.
	- Trojan asteroids
	- Coorbital motion of Janus and Epimetheus (atellites of Saturn)
	- Etc.

### Existence of equilibrium points for the RTBP
Take $x_{1}= x$, $x_{2}=y$, $x_{3}= x'$, $x_{4}= y'$, the system (S) becomes
$$\begin{cases}
\frac{dx_{1}}{dt}= x_{1}' = x_{3} \\
\frac{dx_{2}}{dt}= x_{2}' = x_{4} \\
\frac{dx_{3}}{dt}= x_{3}' = 2x_{4} + \Omega_{x_{1}} \\
\frac{dx_{4}}{dt}= x_{4}' = -2x_{3} + \Omega_{x_{2}} \\
\end{cases}$$
This is the system of ODE's of first order we are going to implement. 

###### Def | ODE reformulation

$$\begin{cases}
x_{1}' = x_{3} \\
x_{2}' = x_{4} \\
x_{3}' = 2x_{4} + \Omega_{x_{1}} \\
x_{4}' = -2x_{3} + \Omega_{x_{2}} \\
\end{cases} \qquad \Leftrightarrow \qquad X' = F(X)$$
**Equilibrium points**: $F(X) = 0$, $x_{3}=x_{4}=0$

$$\begin{cases}
\Omega_{x_{1}} = 0  \\
\Omega_{x_{2}} = 0
\end{cases} \qquad \Leftrightarrow \begin{cases}
\Omega_x = 0  \\
\Omega_y = 0
\end{cases}$$
So,
$$\begin{cases}
\Omega_x = 0  \Leftrightarrow x - \frac{(1-\mu)(x-\mu)}{r_{1}^{3}} - \frac{\mu(x-\mu + 1)}{r_{2}^{3}} = 0\\
\Omega_{y} = 0 \Leftrightarrow y\left[ 1- \frac{(1-\mu)}{r_{1}^{3}} - \frac{\mu}{r_{2}^{3}}\right] = 0
\end{cases}$$
We distinguish two cases:

#### Case a: $y\neq 0$
![[RTBP_L4|300]]

From the 2nd eq, necessarily we have $$1- \frac{(1-\mu)}{r_{1}^{3}} - \frac{\mu}{r_{2}^{3}} = 0$$
From the 1st eq: $$x\left( 1- \frac{(1-\mu)}{r_{1}^{3}} - \frac{\mu}{r_{2}^{3}}\right) + \frac{\mu(1-\mu)}{r_{1}^{3}} - \frac{\mu(1-\mu)}{r_{2}^{3}} = 0$$
The first term is 0 (from the eq above), so we have that if $\mu(1-\mu) \neq 0$:
$$ \frac{1}{r_{1}^{3}}- \frac{1}{r_{2}^{3}} = 0 \Leftrightarrow r_{1}^{3} = r_{2}^{3} \Leftrightarrow r_{1} = r_{2}$$
Then from the first condition we get:
$$1-\frac{1-\mu}{r^{3}} - \frac{\mu}{r^{3}} = 1 - \frac{1}{r^{3}} = 0 \Leftrightarrow r^{3}=1$$
So we have, $r=1$ as equilibrim point.

This means we have an equilateral triangle. Upwards (L4) and downwards (L5).

$L_{4}, L_{5}$ are called the triangular (or equilateral) equilibrium points: $L_{4,5} = (x_{1},x_{2},x_{3},x_{4}) = (\mu-\frac{1}{2}, \frac{\pm\sqrt{3}}{2}, 0, 0)$

#### Case b: $y = 0$

Remember,
$$\begin{cases}
\Omega_x = 0  \Leftrightarrow x - \frac{(1-\mu)(x-\mu)}{r_{1}^{3}} - \frac{\mu(x-\mu + 1)}{r_{2}^{3}} = 0\\
\Omega_{y} = 0 \Leftrightarrow y\left[ 1- \frac{(1-\mu)}{r_{1}^{3}} - \frac{\mu}{r_{2}^{3}}\right] = 0
\end{cases}$$
So, the 2nd equation is satified automatically. We need to solve only the first one.

Also, the position vectors are now

$$\begin{cases}
r_{1} &= \sqrt{(x-\mu)^{2}} \\
r_{2} &= \sqrt{(x-\mu + 1)^{2}}
\end{cases}$$
We will distinguish 3 different cases:

##### Case b.1: $L_{2}$
![[RTBP_L2]]

Those equilibrium points on the $x$-axis located on the left handside of $P_2$, at $\xi$ distance from $P_2$:

$$\begin{cases}
x &= \mu - 1-\xi \\
r_{1} &= 1 + \xi \\
r_{2} &= \xi
\end{cases}$$
We plug this into the previous expressions:

$$\begin{aligned}
0 =& x - \frac{(1-\mu)(x-\mu)}{r_{1}^{3}} - \frac{\mu(x-\mu + 1)}{r_{2}^{3}} \\
0 =& \mu-1 - \xi + \frac{(1-\mu)(1+\xi)}{(1+\xi)^{3}} - \frac{\mu\xi}{\xi^{3}}
\end{aligned}$$
Multiplying by $(1+\xi)^{2}\xi^{2}$, we obtain

###### Euler quintic polynomial equation

$$\xi^{5}+ (3-\mu)\xi^{4} + (3-2\mu)\xi^{3} - \mu\xi^{2} - 2\mu\xi - \mu = 0$$
*Eq(EL2)*

We want all the possible roots with $\xi> 0$.

In order to prove that there exists a unique  $\xi > 0$:
1. First, we use [[Descartes' rule]]: The number of **positive roots** of a polynomial is less or equal than the number of sign changes in the sequence given by the coefficients of the polynomial.
	*Coefficients:* $1, \; 3-\mu, \; 3-2\mu, \; -\mu, \; -2\mu, -1$
	1 single change of sign from $3-2\mu$ to $-\mu$  (remember $\mu \in (0, \frac{1}{2})$), which means the number of positive roots is $\leq 1$.
2. Second, we apply [[Bolzano's theorem]]:
	$$\begin{cases}
 P(0) = -\mu < 0  \\
P(1) = 7-7\mu=7(1-\mu) > 0
\end{cases}$$
	To find that there's at least one root between $0$ and $1$.

So, we will have $L_{2}=(\mu-1-\xi, 0, 0, 0)$.

###### Numerical computation of $\xi$
> V. Szebehly's book

One way is to rewrite [[#Euler quintic polynomial equation]] as
$$\xi^{3}= \frac{\mu(1+\xi)^{2}}{3-2\mu + \xi(3-\mu + \xi)} \quad \Leftrightarrow \quad \xi= \left[\frac{\mu(1+\xi)^{2}}{3-2\mu + \xi(3-\mu + \xi)}\right]^{\frac{1}{3}} = f_{2}(\xi)$$
We take an initial $\xi_{0}$ and we compute the sequence:
$$\xi_{0}, \; \xi_{1}=f_{2}(x_{0}), \; \xi_{2}=f_{2}(x_{1}), \; \dots \; \xi_{n+1}=f_{2}(x_{n}), \; \dots$$
We stop the procedure when $|f(\xi) - \xi| < tol$.

*What value of $\xi_{0}$ do we take?*

We write *(EL2)* as

$$\left(\frac{\mu}{3(1-\mu)}\right)^\frac{1}{3}= \left(\frac{\xi^{3}(1+\xi+\xi^{2}/3)}{(1+\xi)^{2}(1-\xi)^{3}}\right)^\frac{1}{3}$$
which is equivalent to saying
$$\nu = F(\xi) \Leftrightarrow \xi = F^{-1}(\nu) = g(\nu) = g'(0)\nu + \dots = \nu + \dots$$
We, thus, take as $\xi_{0}=\nu = \left(\frac{\mu}{3(1-\mu)}\right)^{\frac{1}{3}}$.

##### Case b.2: $L_{1}$
![[RTBP_L1|300]]
We look for those equilibrium points that are between $P_{1}$ and $P_{2}$. It's at $\xi$ distance from $P_{2}$

$$\begin{cases}
x &= \mu - 1 + \xi \\
r_{1} &= 1 - \xi \\
r_{2} &= \xi
\end{cases}$$
We plug this into the previous expressions:
$$\begin{aligned}
0 =& x - \frac{(1-\mu)(x-\mu)}{r_{1}^{3}} - \frac{\mu(x-\mu + 1)}{r_{2}^{3}} \\
0=& \mu-1 + \xi + \frac{(1-\mu)(1-\xi)}{(1-\xi)^{3}} - \frac{\mu\xi}{\xi^{3}}
\end{aligned}$$
###### Euler quintic polynomial equation

$$Q(\xi) = \xi^{5} - (3-\mu)\xi^{4} + (3-2\mu)\xi^{3} - \mu\xi^{2} + 2\mu\xi - \mu = 0$$
*Eq(EL1)*

We look for roots $\xi \in (0, 1)$.

We do
$$\begin{cases}
Q(0) &= -\mu < 0 \\
Q(1) &= 1 - \mu > 0
\end{cases}$$
By [[Bolzano's theorem]], there exists at least one root $\xi \in (0, 1)$. Actually, $\exists !$ root (to be checked numerically).

There exists a unique equilibrium point between $P_{1}$ and $P_{2}$:
$$L_{1}=(\mu-1+\xi, 0, 0, 0).$$
###### Numerical computation of $\xi$
We move from a polynomial equation to a fix point equation as before
$$\xi= \left[\frac{\mu(1-\xi)^{2}}{3-2\mu - \xi(3-\mu - \xi)}\right]^{\frac{1}{3}} = f_{1}(\xi)$$
and we will have $\xi = f_{1}(\xi)$

We do the same procedure as before. For the initial value of  $\xi_{0}=\nu = \left(\frac{\mu}{3(1-\mu)}\right)^{\frac{1}{3}}$.

##### Case b.3: $L_{3}$
![[L3_RTBP]]
We look for those equilibrium points that on the right hand side of $P_{1}$It's at $\xi$ distance from $P_{1}$

$$\begin{cases}
x &= \mu + \xi \\
r_{1} &= \xi \\
r_{2} &= 1 + \xi
\end{cases}$$
We plug this into the previous expressions:
$$\begin{aligned}
0 =& x - \frac{(1-\mu)(x-\mu)}{r_{1}^{3}} - \frac{\mu(x-\mu + 1)}{r_{2}^{3}} \\
0=& \mu + \xi - \frac{(1-\mu)\xi}{\xi^{3}} - \frac{\mu(1+\xi)}{(1+\xi)^{3}}
\end{aligned}$$
###### Euler quintic polynomial equation

$$R(\xi) = \xi^{5} + (2+\mu)\xi^{4} + (1+2\mu)\xi^{3} - (1-\mu)\xi^{2} + 2(1-\mu)\xi - (1-\mu) = 0$$
*Eq(EL3)*

We look for roots $\xi \in (0, 1)$.

By Descartes rule, theres only one change of sign, so the number of positive roots is $\leq 1$. By Bolzano's rule,
$$\begin{cases}
R(0) &= -(1 - \mu) < 0 \\
Q(1) &= 7\mu > 0
\end{cases}$$
so at least $\exists$ one root.

There exists a unique equilibrium at the right hand side of $P_{1}$:
$$L_{3}=(\mu+\xi, 0, 0, 0).$$
with $\xi \in (0, 1)$

###### Numerical computation of $\xi$
As before
$$\xi= \left[\frac{(1-\mu)(1+\xi)^{2}}{1+2\mu + \xi(2+\mu + \xi)}\right]^{\frac{1}{3}} = f_{3}(\xi)$$
and we will have $\xi = f_{3}(\xi)$

For the initial value, we proceed as follow:

Our quintic polynomial equation is $R(\xi) = 0$ with $\xi \in (0, 1)$. Numerically, one can check that $\xi$ is closed to 1, so we do the change of variables: $\eta = \xi - 1$.  We obtain this new quintic:
$$\eta^{5} + (7+\mu)\eta^{4} + (19+6\mu)\eta^{3} + (24+13\mu)\eta^{2} + 2(6+7\mu)\eta + 7\mu = 0$$
or $$\eta\left[12 + 14\mu + (24+13\mu)\eta + (19+6\mu)\eta^{2}+(7+\mu)\eta^{3} + \eta^{4}  \right]= -7\mu$$
So, $$\eta = \frac{-7\mu}{12 + 14\mu + O(\eta)} = \frac{-7\mu}{12+14\mu}(1+O(\eta)) = \frac{-7\mu}{12}(1+O(\eta))(1+O(\eta))$$and then $$\xi_{0}= 1 - \frac{7\mu}{12}$$
#### Summary
In summary, the RTBP has 5 equlibium points:
- $L_{1, 2, 3}$ the **collinear** ones
-  $L_{4, 5 }$ the **triangular** ones.

### Stability of equilibrium points ($L_{i}, \quad i=1,\dots, 5$)
Let us compute the eigenvalues of $DF(L_{i})$

$$DF|_{L_{i}} = \begin{pmatrix}0 & 0 & 1 & 0 \\ 
0 & 0 & 0 & 1 \\ 
\Omega_{xx} & \Omega_{xy} & 0 & 2 \\ 
\Omega_{yx} & \Omega_{yy} & -2 & 0
\end{pmatrix}$$
The [[characteristic polynomial]] is $\det{(DF(L_{i}) - \lambda \mathbb{I})} = 0$, or equivalently
$$\lambda^{4} + (4-\Omega_{xx}(L_{i}) - \Omega_{yy}(L_{i}))\lambda^{2} + \Omega_{xx}(L_{i})\Omega_{yy}(L_{i}) - [\Omega_{xy}(L_{i})]^{2} = 0$$

#### For $L_{1}, L_{2}, L_{3}$
Recall $$\Omega(x, y) = \frac{1}{2}(x^{2}+ y^{2}) + \frac{1-\mu}{r_{1}} + \frac{\mu}{r_{2}}+ \frac{1}{2}\mu(1-\mu) $$ and $$\begin{align*}
\Omega_{xx}&=1 - \frac{1-\mu}{r_{1}^{3}} + \frac{3(1-\mu)(x-\mu)^{2}}{r_{1}^{5}} - \frac{\mu}{r_{2}^{3}}+ \frac{3\mu(x-\mu+1)^{2}}{r_{2}^{5}}\\
\Omega_{xy} &= y\left(\frac{3(1-\mu)(x-\mu)}{r_{1}^{5}} + 3\mu\frac{x-\mu+1}{r_{2}^{5}}\right)\\
\Omega_{yy} &= 1 - \frac{1-\mu}{r_{1}^{3}} - \frac{\mu}{r_{2}^{3}}+ y^{2}\left(\frac{3(1-\mu)}{r_1^5}+ \frac{3\mu}{r_2^{5}}\right)\end{align*}$$
###### Lemma
$$\begin{align*}
\Omega_{xx}(L_{i}) &=  1 + 2\frac{1-\mu}{|x-\mu|^{3}} + \frac{2\mu}{|x-\mu+1|^{3}}>0 \\
\Omega_{xy}(L_{i}) &= 0\\
\Omega_{yy}(L_{i}) &< 0 \qquad \textrm{(To be checked numerically)}
\end{align*}$$
So the characteristic equation becomes
$$\lambda^{4} + (4-\Omega_{xx}(L_{i}) - \Omega_{yy}(L_{i}))\lambda^{2} + \Omega_{xx}(L_{i})\Omega_{yy}(L_{i}) = 0$$

Now, we define:
$$\begin{cases}
\beta_{1} &= 2 - \frac{(\Omega_{xx}+\Omega_{yy})|_{L_{i}}}{2} \quad\longleftarrow 2\beta_{1} = 4-(\Omega_{xx}+\Omega_{yy})|_{L_{i}} \\
\beta_{2}^{2} &=-(\Omega_{xx}\cdot\Omega_{yy})|_{L_{i}}
\end{cases}$$ and we can rewrite the characteristic equation as:
$$\lambda^{4} + 2\beta_{1}\lambda^{2}-\beta_{2}^{2}= 0 \Rightarrow \lambda^{2}= -\beta_{1} \pm \sqrt{\beta_{1}^{2}+ \beta_{2}^{2}}$$
Since $|\beta_{1}^{2}+ \beta_{2}^{2}| > |\beta_{1}|$, it means that we will have that the square root is bigger so we have two kind of solutions:
$$\lambda^{2}= \begin{cases}
A > 0 \\
B < 0
\end{cases}$$
and thus $$\Rightarrow \lambda = \begin{cases}
\quad\sqrt{A} > 0  \\
- \sqrt{A} < 0  \\
\quad \sqrt{-B}i \\
-\sqrt{-B}i
\end{cases}$$
This is going to be called **center x saddle**, center for the imaginary eigenvalues and and saddle for the real, positive and negative points.  (check picture).

So $\forall u \in (0, \frac{1}{2})$, $L_{1}, L_{2}, L_{3}$ are unstable for the original nonlinear system (the RTBP).

> For any $\mu \in (0, \frac{1}{2}]$, there exists:
> - a 1d unstable manifold $W^{u}(L_{i})$
> - a 1d stable manifold $W^{s}(L_{i})$

#### For $L_{4}, L_{5}$
For $L_{4, 5} = (\mu-\frac{1}{2}, \pm \frac{\sqrt{3}}{2}, 0, 0)$, we compute:
$$\begin{align*}
\Omega_{xx}(L_{4}) = \Omega_{xx}(L_{5})= \frac{3}{4}\\
\Omega_{yy}(L_{4}) = \Omega_{yy}(L_{5})= \frac{9}{4}\\
\Omega_{xy}(L_{4}) = \frac{3\sqrt{3}}{2}\left(\mu - \frac{1}{2}\right)= - \Omega_{xy}(L_{5})
\end{align*}$$
> checking this is an exercise

We obtain $$\lambda^{4}+ \lambda^{2}+ \frac{27}{4}\mu (1-\mu) = 0$$so that $$\lambda^{2}= \frac{1}{2}\left(-1 \pm \sqrt{1 - 27\mu(1-\mu)}\right)$$Now let's discuss the sign of the inside of the root, which we will define as:
$$f(\mu) = 1-27\mu(1- \mu) = 27\mu^{2}-27\mu+1, \quad \mu\in (0, 1/2]$$
![[../../Media/Pasted image 20221102164231.png]]
We are interested in the point where the graph crosses the x-axis: $\mu_{R}$:
$$f(\mu_{R}) = 0 \rightarrow 27\mu^{2} - 27\mu+1 = 0 \Rightarrow \mu_{R}=\frac{1}{2}\left(1\pm\frac{\sqrt{69}}{9}\right)$$
since $\mu \in (0, 1/2]$, then we take the minus part:
$$\mu_{R}=\frac{1}{2}\left(1-\frac{\sqrt{69}}{9}\right) = 0.038...$$
We distinguish 3 cases:

###### Case 1: $0<\mu<\mu_{R}$
$$\lambda^{2}= \begin{cases}
\Lambda_{1} < 0  \\
\Lambda_{2} < 0
\end{cases} \Rightarrow \lambda = \begin{cases}
\pm \sqrt{|\Lambda_{1|}}i = \pm w_{1}i \\
\pm \sqrt{|\Lambda_{2|}}i = \pm w_{2}i
\end{cases}$$
with 
$$\begin{align*}
w_{1}= \left(\frac{1}{2}|-1 - \sqrt{1 - 27\mu(1-\mu)}|\right)^{\frac{1}{2}}= \frac{1}{\sqrt{2}}\sqrt{1 + \sqrt{1 - 27\mu(1-\mu)}}\\
w_{2}= \left(\frac{1}{2}|-1 + \sqrt{1 - 27\mu(1-\mu)}|\right)^{\frac{1}{2}}= \frac{1}{\sqrt{2}}\sqrt{1 - \sqrt{1 - 27\mu(1-\mu)}}
\end{align*}$$
so that $\omega_{1}^{2}> \frac{1}{2}>\omega_{2}^{2}$
> Picture with plot, all points in the y-axis![[2.1. The 3 body problem 2022-11-15 12.31.55.excalidraw]]

In this case we have a **center x center**: we have no info about the stability for the RTBP.

###### Case 2: $\mu=\mu_{R}$
$\lambda^{2}= \frac{-1}{2}\Rightarrow \lambda = \pm \frac{1}{\sqrt{2}}i$

> Picture with plot, all points in the y-axis

This is a **degenerate center x center** ($\omega_{1}= \omega_{2}=\omega$)

###### Case 3: $\mu_{R}<\mu<1/2$
$$\lambda^{2}= \frac{-1\pm ai}{2} \Rightarrow \lambda = \begin{cases}
\quad\lambda_{1} \\
\quad\bar{\lambda}_{1} \\
-\lambda_{2} \\
-\bar{\lambda}_{2}
\end{cases} $$
> This is a **complex saddle**:
> 	-There exists a 2d unstable manifold $W^{u}(L_{4,5})$
> 	-There exists a 2d stable manifold $W^{s}(L_{4,5})$

It's unstable.

###### How to compute it numerically?
We have a tangent plane, we take a circle of initial conditions around the point and integrate forward/backward in time.

###### Remark
Another very important consequence of the type of eigenvalues is the existence of periodic orbits, guaranteed by Lyapunov Theorem:

##### Lyapunov Theorem
> Ref Meyer-Hall-Offin book

Assume that a system of ODE: $$\vec{x}' = \vec{f}(\vec{x}), \quad \vec{x}\in U\subset \mathbb{R}^{n}$$has a nondegenerate first integral $H(\vec{x})$ (that is, $\nabla H(\vec{r}) \neq 0$ for $\vec{r}$ a regular point), and an equilibrium point with chaaracteristic exponents $\pm i\omega, \lambda_{3}, \dots, \lambda_{n}$.

If $\frac{\lambda_{j}}{i\omega} \notin \mathbb{Z}$, $j=3, \dots, n$, then there exists a one-paramter family of periodic orbits emanating from the equilibrium point. Moreover, when approaching the equilibrium point along the family, the period tends to $\frac{2\pi}{\omega}$.

> If I give the value of one parameter (which will be the first integral), then I can identify the orbit.

##### Application to the RTBP
$$\vec{X}' = \vec{F}(\vec{X}) \quad \vec{X}\in U\subset\mathbb{R}^{4}$$
First integral: $C(x, y, x', y') = 2\Omega(x, y) - (x'^{2}+y'^{2})$ ([[Jacobi first integral]]).
*Check: $\nabla C = (2 \Omega_{x}, 2 \Omega_{y}, -2x', -2y') = \vec{0} \Longleftrightarrow \Omega_{x}= \Omega_{y}=x'=y' = 0 \Longleftrightarrow L_{i}, i=1, \dots, 5$ 

###### For $L_{1}, L_{2}, L_{3}$
Eigenvalues: $\pm i \omega, \pm \lambda$, with $\lambda \in \mathbb{R}$, we check
$$\frac{\lambda}{i \omega} \notin \mathbb{Z}$$since $\lambda$ is always real and divided by an imaginary number it will never be an integer number.
$\Rightarrow$ for any value of $\mu$, there exists a one-parameter family of periodic orbits emanating at $L_{1,2,3}$ and the period of the periodic orbits tend to $\frac{2\pi}{\omega}$ (when approaching $L_{i}$)
> Check picture

###### For $L_{4}, L_{5}$
- **Case: $\mu = \mu_{R}$**, 
	then $\omega_{1}=\omega_{2}=\omega$, so the coefficient will be 1, an integer number.
- **Case: $\mu_{R}<\mu<1/2$**
	we don't have exponents in the form of $\pm i \omega$, so I cannot apply the formula.
- **Case : $0 < \mu < \mu_{R}$**
	eigenvalues $\pm i\omega_{1}, \pm i\omega_{2}$ ($\omega_{1}>\omega_{2}, \, \omega_{1}^{2}> \frac{1}{2}>\omega_{2}^{2}$).
	- **First case**
		We have $0 <\frac{ \pm i \omega_{2}}{i\omega_{1}} = \frac{\omega_{2}}{\omega_{1}} < 1$ (since $\omega_{1}>\omega_{2}$) , then $\frac{\pm i \omega_{2}}{i\omega_{1}} \notin \mathbb{Z} \Rightarrow$ There exists a one-parameter family of periodic orbits emanating at $L_{4}$ and $L_{5}$ and the period tends to $2\pi/\omega_{1}$: the so called family of **Lyapunov periodic orbits of short period** .  
	- **Second case**
		We have $\frac{ \pm i \omega_{2}}{i\omega_{1}} = \frac{\omega_{2}}{\omega_{1}} \notin \mathbb{Z}$
		Let us show that this is true for $\mu \neq \mu_r$, $\mu_{r}=\frac{1}{2}-\frac{1}{2}\left(\frac{1-16r^2}{27(r^{2}+1)^{2}}\right)^{\frac{1}{2}}$, for $r=1, 2, 3...$ then $\frac{\omega_{1}}{\omega_{2}\notin}\mathbb{Z}$.
		We assume now $\frac{\omega_{1}}{\omega_{2}}$, which is equivalent to
		$$\frac{\frac{1}{\sqrt{2}}\sqrt{1+x}}{\frac{1}{\sqrt{2}}\sqrt{1-x}}= r$$
		where $x = \sqrt{1-27\mu(1-\mu)}$ 
		Same as,
		$$\frac{1+x}{1-x}=r^{2} \Leftrightarrow x = \frac{r^{2}-1}{r^{2}+1} \Leftrightarrow \mu^{2}-\mu + \frac{4r^{2}}{27(r^{2}+1)^{2}}=0$$
		same as
		$$\mu = \frac{1}{2}\left(1 \pm \sqrt{1- \frac{16r^{2}}{27(r^{2}+1)}}\right)$$
		Since $\mu$ must $\mu\in(0, 1/2]$, then it means that the values of $\mu$ for which we have an integer ratio are $$\mu_{r} = \frac{1}{2} - \frac{1}{2}\left(1- \frac{16r^{2}}{27(r^{2}+1)}\right)^\frac{1}{2}$$
		If $\mu \neq \mu_{r}$, $r=1, 2...$ then there exists a one-parameter family of Lyapunov periodic orbits emanating at $L_{4,5}$ and the period tends to $\frac{2\pi}{\omega_{2}}$when approaching $L_{4,5}$: the so called **Lyapunov family of periodic orbits of long period**.
		
	> So, when $\mu$ is different from $\mu_{r}$, then the ratio won't be an integer ratio. We will demonstrate the opposite.

#### Recap: Computation of unstable manifolds taking the linear approximation
![[Unstable_manifold_computation]]
We have a circle of initial conditions:
$$\begin{cases}
s_{1} &= r \cos{\theta} \\
s_{2} &= r \sin{\theta}
\end{cases}$$
for $\theta \in [0, 2\pi]$ and $r$ small and for each initial condition we integrate forward in time. However, we will see a more precise way to do this.
