---
aliases: [parametrization of invariant manifolds, Expansion of parametrizations of invariant manifolds]
subject: Numerical Methods for Dynamical Systems
lecturer: Mercè Ollé Torner
format: in-person
program: Master in Advanced Mathematics and Mathematical Engineering
dates: 
tags: #mamme #numericalmethods #dynamicalsystems
---
Motivation: [[Motivation for expansion of parametrizations of invariant manifolds (for flows)]]

## 2.2. Expansion of parametrizations of invariant manifolds (for flows)
> **Reference**: *The parametrization method for invariant manifolds* Alex Haro, Marta Canadell, Jordi Lluís Figueras, ALejandro Luque, Josep M. Mondelo.
> **Theoretical background**: Xavier Cabré, Rafel de la Llave, Ernest Fontich (3 papers)

### Motivation
Assume $Z' = G(Z)$ as system of $n$ ODE, $Z \in U \subset \mathbb{R}^{n}$, $Z_0$ an equilibrium point  such that the eigenvalues of $DG(Z_0)$ are $\lambda_{1}, \lambda_{2}, \dots, \lambda_{n}$ with $\lambda_{1}, \lambda_{2} > 0$. We know, thus, there exists a 2d unstable invariant manifold.

- For the linearized system, we take the $\vec{v}_{1}^{u}, \vec{v}_{2}^{u}$ eigenvectors. If $\lambda_{2}> \lambda_{1} > 0$, then $\lambda_{2}$ is the fast  dimension. The whole plane is the unstable manifold.
	![[linear_Wu|200]]
- For the non-linear original system, we have a 2d invariant manifold, $W^{u}$.
	$$Z_{0} = Z_{0} + s_{1}\vec{v}_{1}^{u} + s_{2}\vec{v}_{2}^{u}$$
	with $$\begin{cases}
s_{1} &= r\cos{\theta} \\
s_{2} &= r\sin{\theta}
\end{cases}$$
	with $r$ *very* small and integrate forward in time. That's how we typically do it.
	
See [[Motivation for expansion of parametrizations of invariant manifolds (for flows)]] and [Jupyter Notebook](http://localhost:8888/notebooks/UPC/MAMME/NMD/Assignments/Motivation%20-%20parametrizations%20of%20invariant%20manifolds.ipynb) for more.

### Goal
To obtain a high order power expansion for a parametrization of invariant manifolds of an equilibrim point of a vector field.

Let us start $Z' = G(Z)$, $Z_0$ equilibrium point, $Z \in U \subset \mathbb{R}^{n}$. Assume $G(Z_{0)}= 0$, and the following eigenvalues:
$$P^{-1}DG(Z_{0})P = \begin{pmatrix}\lambda_{1} & \dots  \\  & \ddots  &   \\  & \cdots & \lambda_{n}\end{pmatrix}$$
We do a change of variables: $z = Z_{0} + P \cdot z$. We obtain
$$z' = F(z),$$
where $F(z) = P^{-1}G(Z_{0}+P\cdot z)$.
> $Z' = P z' \Rightarrow z' = P^{-1}Z' = P^{-1}G(Z) = P^{-1}G(Z_{0}+ P\cdot z)$

Now $F(0) = 0$, $DF(0) = P^{-1}DG(Z_{0)P}= \begin{pmatrix}\lambda_{1} & \dots  \\  & \ddots  &   \\  & \cdots & \lambda_{n}\end{pmatrix}$
My input used to be $Z_{0}, G$ and now it's $F$.

We consider the Taylor expansion:
$$F(z) = DF(0)z + F_{2}(z) + F_{3}(z) + \dots$$
and this will be my input. Notice that $F_{2}, F_{3}$ are the 2nd, 3rd order terms.

Now we have this input and we want to compute the invariant manifold of this zero. 

We choose the first $d$ eigenvalues of $DF(0)$ (we can always reorder them) and let $V^{d}$ be a $d$dimensional linear subspace spanned by the $d$ eigenvectors. (Assume, for example, that $\lambda_{1\dots d}>0$ $\Rightarrow$ there exists a $d$-dimensional unstable invariant manifold $\mathfrak{W}^u$ *(this is a gothic W)*)

Our goal is to obtain a high order approximation of the $d$-dimensional manifold $\mathfrak{W}^u$ for system $z' = F(z)$ tangent to $V^{d}$

In our example, $W(s) = \begin{pmatrix}v_{1}^{1} & v_{1}^{2} & \dots & v_{1}^{d} \\ \vdots & \vdots  & & \vdots  \\ v_{n}^{1} & v_{n}^{2} & \dots & v_{n}^{d}\end{pmatrix} \begin{pmatrix}s_{1}  \\ \vdots  \\ s_{d}\end{pmatrix} = s_{1}\vec{v}^{1}+\dots +s_{d}\vec{v}^{d} = \begin{pmatrix}v_{1}^{1} & v_{1}^{2} & \dots & v_{1}^{d}  & \cdots \\ \vdots & \vdots  & & \vdots &   \\ v_{n}^{1} & v_{n}^{2} & \dots & v_{n}^{d} & \cdots\end{pmatrix}\begin{pmatrix}s_{1}  \\ \vdots  \\ s_{d} \\ 0  \\ \vdots \\ 0 \end{pmatrix}$
where the last matrix is $P$.

With the original variables $W(s) = Z_{0}+ P(\begin{pmatrix}s_{1} \\ \vdots \\ s_{d} \\ 0 \\ \vdots \\  0 \end{pmatrix}) = Z_{0}+s_{1}\vec{v}^{1}+\dots +s_{d}\vec{v}^{d}$.
This is an approximation for parametrizing the plane. But we are not interested in the plane now, only in the "border".
![[parametrization_nmds|200]]

More concretely, we look for a parametrization
$$\begin{align*}
W: \tilde{U}\subset \mathbb{R}^{d} &\longrightarrow \mathbb{R}^n\\
s &\longrightarrow W(s) = z
\end{align*}$$
of the invariant manifold $\mathfrak{W}$ where $s = (s_{1}, \dots, s_{d})$ are the coordinates (parameters) of the parametrization and $W(0) = 0$. The internal dynamics on the manifold is described by a vector field
$$s' = f(s)$$
I have two flows, one for $z' = F(z)$, $\Phi_{t}$ and one for $s'=f(s)$, $\phi_{t}$, with $f(0) = 0$.

So, we look for $W$ and $f$ such that is invariant by the flow of $F$:
1. $\{W(s)\}_{s\in \tilde{W}\subset \mathbb{R}^{d}}$ is invariant by the flow of $F$.
2. the internal dynamics of $s$ is given by $s' =f(s)$
That is, we want
$$\Phi_{t}(W(\tilde{s})) = W(\phi_{t}(\tilde{s}))$$

Let us take $\frac{d}{dt}$:
$$F(\Phi_{t}(W(\tilde{s}))) = DW(\phi_{t}(\tilde{s}))\cdot f(\phi_{t}(\tilde{s}))$$

> we have that $\phi_{t}(\tilde{s}) = s$ and $\Phi_{t}(W(\tilde{s})) = W(s)$.
 
that is we want $W(s)$, $f(s)$ such that
###### Def: Invariance equation
$$F(W(s)) = DW(s)f(s)$$
And, conversely, if the invariance equation is true, then (IC) is also tre (It can be proved).

So, what we will do is to solve the invariance equation. 

A geometrical interpretation ![[geometrical_interpretation]]

Unknowns: $W(s), f(s)$ and known is $F$


# The parametrization method
*Date*: 16-11-2022
We have
$$\begin{align*}
Z' &= G(Z), \quad Z_{0} \textrm{: an equilibrim point}\\
Z &= Z_{0}+Pz
\end{align*}$$ and we transform it so that $$z' = F(z)$$ with 0 an equilibrium point: $F(0) = 0$, $DF(0) = \begin{pmatrix}\lambda_{1} & &  \\  & \ddots  &  \\  & & \lambda_{n}\end{pmatrix}$
And we will do the expansion:
$$F(z) = DF(0)z + F_{2}(z) + F_{3}(z) + \ldots = F_{1}(z) + F_{2}(z) + F_{3}(z) + \ldots$$
and $F_{1}=\begin{pmatrix}\lambda_{1}z_{1} \\ \vdots  \\ \lambda_{n}z_{n}\end{pmatrix} + \sum\limits_{k\geq2}F_{k}(z)$
For example
$$DF(0) = \begin{pmatrix}\lambda_{1}>0 & & & & \\ & \ddots & &  &  \\  & & \lambda_{d}>0 & &\\  & & &\lambda_{d+1}<0 & & &\\  & & & &\ddots & & \\  & & & & & &\lambda_{n}<0\end{pmatrix}$$
There exists a d-dimensional unstable manifold

**Specific goal**: we look for a d-dim manifold, so we want:
$$W(s) = \sum\limits_{k\geq1}W_{k}(s) = \begin{pmatrix}s_{1} \\ \vdots  \\ s_{d} \\ 0 \\ \vdots \\ 0\end{pmatrix} + \sum\limits_{k\geq2}W_{k}(s); \qquad f(s) = \begin{pmatrix}\lambda_{1}s_{1} \\ \vdots  \\ \lambda_{d}s_{d} \end{pmatrix} + \sum\limits_{k\geq2}f_{k}(s)$$
where $(s_{1}, \ldots, s_{d}, 0, \ldots, 0)$ is $W_{1}(s)$ and $W(0) = 0$, $f_{1} = (\lambda_{1}s_{1}, \dots)$ and $f(0) = 0$
that are solution of the invariance equation (eq 4)
$$F(W(s)) = DW(s)\cdot f(s)$$
which comes from $\phi_{t}(W(s)) = W(\phi_{t}(s))$.

###### Remark 1
Taking $W(s)$ and $f(s)$ as above the invariance equation (4) is satisfied at first order:
$$[F(W(s))]_{1} = F_{1}(W_{1}(s)) = F_{1}\begin{pmatrix}s_{1} \\ \vdots  \\ s_{d} \\ 0 \\ \vdots \\ 0\end{pmatrix} = \begin{pmatrix}\lambda_{1}s_{1} \\ \vdots  \\ \lambda_{d}s_{d} \\ 0 \\ \vdots \\ 0\end{pmatrix}$$
$$[DW(s)f(s)]_{1}=DW_{1}(s)f_{1}(s) = \begin{pmatrix}I_{d\times d \\ 0}\end{pmatrix}\begin{pmatrix}\lambda_{1}s_{1} \\ \vdots  \\ \lambda_{d}s_{d}\end{pmatrix} = \begin{pmatrix}\lambda_{1}s_{1} \\ \vdots  \\ \lambda_{d}s_{d} \\ 0  \\ \vdots  \\ 0\end{pmatrix}$$
so $[F(W(s))]_{1} = [DW(s)f(s)]_{1}$

>We know that $DW_{1}(s)$ is the derivative of the vector $W_{1}$, which is just the $s$ variables and zeros with respect to $s$, so we have $DW_{1}(s) \in \mathbb{R}^{n\times s}$ and we will have an identity matrix stacked with a zero matrix

>Order k of $f$ means order $k$ of z means a homogeneous polynomial of degree k.
>$[F]_1$ means expansion of order 1

###### Remark 2
Once we have done the procedure and we have obtained the parametrization$W(s)$ up to a given order, that is $z = W(s)$
we apply the **change of variables** in order to obtain the parametrization in original variables:
$$W^{\textrm{orig var}}(s) = Z_{0}+P\cdot W(s)$$
> So we are only gonna focus on $W(s)$

###### Remark 3
**Example 1d**
For example $Z' =G(Z)$, $Z_{0}$ with $DF(0) = \begin{pmatrix}\lambda_{1}>0 &   &   & \\ \lambda_{2} &   &  \\  &   &  \ddots  &  \\  &   &   & \lambda_{n}\end{pmatrix} \Rightarrow \exists$ a 1d unstable manifold $W^u$
$$P = \begin{pmatrix}v_{1}^{1}  & \cdots & \cdots \\ \vdots &  \cdots & \cdots \\ v_{n}^{1} & \cdots & \cdots \end{pmatrix}$$
if we take $W(s)$ up to first order: $W(s) \approx W_{1}(s) = \begin{pmatrix}s_{1} \\ 0 \\ \vdots  \\ 0\end{pmatrix}$
then in the original variable
$$W^{\textrm{orig variable}}(s) \approx Z_{0}+PW_{1}(s) = Z_{0}+\begin{pmatrix}v_{1}^{1}  & \cdots & \cdots \\ \vdots &  \cdots & \cdots \\ v_{n}^{1} & \cdots & \cdots \end{pmatrix}\begin{pmatrix}s_{1} \\ 0 \\ \vdots  \\ 0\end{pmatrix} = Z_{0}+s_{1}v^{1}$$
which is what we've done so far. 

> Typically for linear approximations $s\in(0, 10^{-6})$

**Example 2d**
$Z' =G(Z)$, $Z_{0}$ with $DF(0) = \begin{pmatrix}\lambda_{1}>0 &   &   & \\ \lambda_{2}>0 &   &  \\  &   &  \ddots  &  \\  &   &   & \lambda_{n}\end{pmatrix} \Rightarrow \exists$ a 2d unstable manifold $W^u$
$$P = \begin{pmatrix}v_{1}^{1}  & v_{1}^2 & \cdots & \cdots \\ \vdots & \vdots &  \cdots & \cdots \\ v_{n}^{1} & v_{n}^2 & \cdots & \cdots \end{pmatrix}$$
if we take $W(s)$ up to first order: $W(s) \approx W_{1}(s) = \begin{pmatrix}s_{1} \\ s_{2} \\ \vdots  \\ 0\end{pmatrix}$
then in the original variable
$$W^{\textrm{orig variable}}(s) \approx Z_{0}+PW_{1}(s) = Z_{0}+\begin{pmatrix}v_{1}^{1} & v_{1}^{2}  & \cdots & \cdots \\ \vdots & \vdots &  \cdots & \cdots \\ v_{n}^{1} & v_{n}^{2} & \cdots & \cdots \end{pmatrix}\begin{pmatrix}s_{1} \\ s_{2} \\ 0 \\ \vdots  \\ 0\end{pmatrix} = Z_{0}+sv^{1} + s_{2}v^{2}$$
which is what we have done so far.

### Resolution of the invariance equation (up to a high order)
$$F(W(s)) = DF(W(s))f(s)$$
###### Notation
We know $F(z)$ (this is my input) where $F_{k}$ means
$$F_{k}^{i}=\sum\limits_{|l|=k=l_{1}+\dots + l_{n}} F^{i}_{k,l}z^{l}=\sum\limits_{|l| = k}F^{i}_{k,l} z_{1}^{l_{1}} \cdots z_{n}^{l_{n}}$$
For the $k$ term, we have $n$ components. Each component $i$ is a homogeneous polynomial of degree $k$ in variables $z_{1, \dots, n}$. 

$$W_{k}^{i}(s) = \sum\limits_{|m|=k=m_{1}+\dots + m_{d}} W^{i}_{k,m}s^{m}=\sum\limits_{|m| = k}W^{i}_{k,l} s_{1}^{m_{1}} \cdots s_{d}^{m_{d}} \qquad i=1, \dots, n$$
For $W(s)$, each term of the expansion $W_{k}$ will have $n$ components and each component is a homogeneous polynomial of  degree $k$ .

$$f_{k}^{i}(s) = \sum\limits_{|m|=k} f^{i}_{k,m}s^{m}=\sum\limits_{|m| = k}f^{i}_{k,l} s_{1}^{m_{1}} \cdots s_{d}^{m_{d}} \qquad i=1, \dots, d$$
and $f$ will have **d** components.

###### Another notation
$z = (x, y)$ where $x$ is the first $d$ components and $y$ are the following $n-d$ components.
$\lambda^{x}$ is the first $d$ eigenvalues
$(\lambda^{x}, m) = \lambda_{1}m_{1}+\dots +\lambda_{d}m_{d}$ is the scalar product.

#### Resolution
We want to solve the invariance equation at order $k$ assuming that it is satisfied up to order $k-1$, that is,
- we know $W_{1}, \dots,  W_{k-1}, f_{1}, \dots, f_{k-1}$ 
- we want $W_{k}, f_{k}$, that is $$W_{k}=\begin{pmatrix}W_{k}^{1} \\ \vdots \\ W_{k}^{n}\end{pmatrix} \quad f_{k}=\begin{pmatrix}f_{k}^{1} \\ \vdots \\ f_{k}^d\end{pmatrix}$$
$$[F(W(s))]_{k}=[DW(s)f(s)]_{k}$$
###### LHS
Let us consider the left hand side terms of order $k$
$$\begin{align*}
[F(W(s))]_{k}&= [F(W_{\leq k})]_{k}=[F(W_{<k} + W_{k})]_{k} =(taylor) = [F(W_{<k})]_{k}+DF(0)W_{k} \\
&= [F(W_{<k})]_{k} + \begin{pmatrix}\lambda_{1} &   &  \\  & \ddots &  \\  &   & \lambda_n\end{pmatrix}\begin{pmatrix}W_{k}^1\\
\vdots \\ W_{k}^n\end{pmatrix}\\
&= [F(W_{<k})]_{k} + \begin{pmatrix}\lambda_{1}W_{k}^{1}\\
\vdots\\
 \lambda_{n}W_{k}^{n}\end{pmatrix}\\
&= (I) + (II)\end{align*}$$
where $(I)$ is known and $(II)$ is unknown
> check at home the first line

###### RHS
Let us consider the right hand side
$$\begin{align*}
[DW(s)f(s)]_{k} &= \sum\limits_{l=0}^{k}[DW]_{l}\cdot [f]_{k-l}= \sum\limits_{l=0}^{k-1}DW_{l+1}\cdot f_{k-l} \\
&=DW_{1}f_{k} + DW_{k}f_{1}+\sum\limits_{l=1}^{k-2}DW_{l+1}f_{k-l}\\
&=DW_{1}f_{k} + DW_{k}f_{1}+\sum\limits_{\tilde{l}=2}^{k-1}DW_{\tilde{l}}f_{k-\tilde{l}+1}\\
&= DW_{1}f_{k} + DW_{k}f_{1}+\sum\limits_{{l}=2}^{k-1}DW_{{l}}f_{k-{l}+1}\\
&= \begin{pmatrix}I\\ 0\end{pmatrix}f_{k} + DW_{k}\begin{pmatrix}\lambda_1s_1\\
\vdots\\ \lambda_{d}s_{d}\end{pmatrix}+\sum\limits_{{l}=2}^{k-1}DW_{{l}}f_{k-{l}+1}\\ &= 
\begin{pmatrix}f_{k}\\ 0\end{pmatrix} + DW_{k}\begin{pmatrix}\lambda_1s_1\\
\vdots\\ \lambda_{d}s_{d}\end{pmatrix}+\sum\limits_{{l}=2}^{k-1}DW_{{l}}f_{k-{l}+1} =  (III) + (IV) + (V)
\end{align*}$$
where $(III), (IV)$ are unknown (because of $f_{k}, DW_{k}$) and $(V)$ is known.

> The first equal is due to $DW, f$ being homogeneous polynomials. The second equal is due to $[DW]_{l}=DW_{l+1}$. Then we also apply that $f_{0}=0$. And $f_{k}, W_{k}$ are unknown.

###### RHS and LHS
$$(I) + (II) = (III) + (IV) + (V) \Longleftrightarrow (IV)-(II)+(III)=(I)-(V)$$
which means:
$$ DW_{k}\begin{pmatrix}\lambda_1s_{1}\\
\vdots\\ \lambda_{d}s_{d}\end{pmatrix} - \begin{pmatrix}\lambda_{1}W_{k}^{1}\\
\vdots\\
 \lambda_{n}W_{k}^{n}\end{pmatrix}+ \begin{pmatrix}f^{1}_{k}\\ \vdots \\ f^{d}_{k} \\ 0  \\ \vdots \\  0\end{pmatrix} = [F(W_{<k})]_{k}+\sum\limits_{{l}=2}^{k-1}DW_{{l}}f_{k-{l}+1} = R_{k} \textrm{ (known)}$$
 Now we expand $W, f, R$ in monomials and notice
 $$\begin{align*}
W_{k}(s) &=  \sum\limits_{|m|=k}W_{k,m}s_{1}^{m_{1}}\dots s_{d}^{m_{d}}\\
\partial_{1}W_{k} &=  \sum\limits_{|m|=k}W_{k,m}s_{1}^{m_{1}-1}\dots s_{d}^{m_{d}}\\
\vdots\\
\partial_{d}W_{k} &=  \sum\limits_{|m|=k}W_{k,m}s_{1}^{m_{1}}\dots s_{d}^{m_{d}-1}\\
\end{align*}$$
and now
$$\begin{align*}
DW_{k}\begin{pmatrix}\lambda_1s_{1}\\
\vdots\\ \lambda_{d}s_{d}\end{pmatrix} &=  \begin{pmatrix}\sum\limits_{|m|=k}W_{k,m}s_{1}^{m_{1}-1}\dots s_{d}^{m_{d}} & \dots  & \sum\limits_{|m|=k}W_{k,m}s_{1}^{m_{1}}\dots s_{d}^{m_{d}-1}\end{pmatrix}\begin{pmatrix}\lambda_1s_{1}\\
\vdots\\ \lambda_{d}s_{d}\end{pmatrix}\\
&= \begin{pmatrix}\sum\limits_{|m|=k}W^{1}_{k,m}s_{1}^{m_{1}-1}\dots s_{d}^{m_{d}} & \dots  & \sum\limits_{|m|=k}W^{1}_{k,m}s_{1}^{m_{1}}\dots s_{d}^{m_{d}-1}\\
\vdots & \cdots & \vdots\\
\sum\limits_{|m|=k}W^{n}_{k,m}s_{1}^{m_{1}-1}\dots s_{d}^{m_{d}} & \dots  & \sum\limits_{|m|=k}W^{n}_{k,m}s_{1}^{m_{1}}\dots s_{d}^{m_{d}-1}\end{pmatrix}\begin{pmatrix}\lambda_1s_{1}\\
\vdots\\ \lambda_{d}s_{d}\end{pmatrix}\\
&= \sum\limits\begin{pmatrix}W_{k,m}^{1}(m_{1}\lambda_{1}+ \dots + m_d\lambda_{d}s^{m}\\ \ldots \\
W_{k,m}^{n}(m_{1}\lambda_{1}+ \dots + m_d\lambda_{d}s^{m}\end{pmatrix} = \sum\limits \begin{pmatrix}W_{k,m}^{i}\\
\vdots\\
W_{k,m}^{n}\end{pmatrix}(\lambda^{x}, m)s^{m}\end{align*}$$

---
*Date: 22-11-2022*
##### Recap:
$$\begin{align*}
Z' &= G(Z) & \qquad(1)\\
Z &=  Z_{0}+ Pz \\
z' &= F(z)  & \qquad(2)
\end{align*}$$
with $Z_0$ an equilibrium point, $F(0) = 0$ and $DF(0) = \begin{pmatrix}\lambda_{1} & \cdots  & 0 \\  \\ 0 & \cdots  & \lambda_{n}\end{pmatrix}$.
**Taylor expansion**:
$$F(z) = F_{1}(z) + F_{2}(z) + \dots = DF(0) + F_{2}+\dots$$
**Invariance equation**
$$\Phi_t(W(s))= W(\phi_{t}(s))$$
and derivative respect $t$:
$$F(W(s)) = DW(s)f(s)$$
**Goal**
$$\begin{align*}
W(s) &=  \begin{pmatrix}s_{1}  \\ \vdots \\ s_{d} \\ 0 \\ \vdots \\ 0\end{pmatrix} + \sum\limits_{k\geq2}W_{k}(s)\\
f(s) &=  \begin{pmatrix}\lambda_{1}s_{1}  \\ \vdots \\ \lambda_{d}s_{d} \end{pmatrix} + \sum\limits_{k\geq2}f_{k}(s)
\end{align*}$$
and after: $W^{\textrm{or var}}(s) = Z_{0}+ PW(s)$.

Last session, we found:

$$DW_{k}\begin{pmatrix}\lambda_{1}s_{1}  \\ \vdots \\ \lambda_{d}s_{d} \end{pmatrix} - \begin{pmatrix}\lambda_{1}W_{k}^{1}  \\ \vdots \\ \lambda_nW_{n}^{d} \end{pmatrix} + \begin{pmatrix}f_{k}^{1} \\ \vdots \\ f_{k}^{d}  \\ 0 \\ \vdots \\ 0\end{pmatrix} = R_k$$
And we can rewrite it as:
$$\sum\limits_{|m|=k} \begin{pmatrix}W_{k,m}^{i}(\lambda^{x}, m)\\
\vdots\\
W_{k,m}^{n}(\lambda^{x}, m)\end{pmatrix}s^{m} - \sum\limits_{|m|=k}\begin{pmatrix}\lambda_{1}W_{k}^{1}  \\ \vdots \\ \lambda_nW_{n}^{d} \end{pmatrix}s_{m}+ \sum\limits_{|m|=k}\begin{pmatrix}f^{1}_{k,m}  \\ \vdots \\ f^{d}_{k,m} \\ 0 \\ \vdots \\ 0 \end{pmatrix}s_{m} = \sum\limits_{|m|=k}\begin{pmatrix}R^{1}_{k,m} \\ \vdots \\ R^{n}_{k,m}\end{pmatrix}s_m$$
and we take common factor:
$$\sum\limits_{|m|=k}\left(\begin{pmatrix}W_{k,m}^{i}(\lambda^{x}, m)\\
\vdots\\
W_{k,m}^{n}(\lambda^{x}, m)\end{pmatrix} - \begin{pmatrix}\lambda_{1}W_{k}^{1}  \\ \vdots \\ \lambda_nW_{n}^{d} \end{pmatrix}+ \begin{pmatrix}f^{1}_{k,m}  \\ \vdots \\ f^{d}_{k,m} \\ 0 \\ \vdots \\ 0 \end{pmatrix}\right)s_m  = \sum\limits_{|m|=k}\begin{pmatrix}R^{1}_{k,m} \\ \vdots \\ R^{n}_{k,m}\end{pmatrix}s_m$$
> We distinguish between the first $d$ components and from the $d+1$-th to the $n$-th component.

##### Equations (components) $i=d+1, \dots, n$
$$\begin{align*}
(\lambda^{x}, m)W_{k,m}^{i} - \lambda_{i}W^{i}_{k,m}&= R^{i}_{k,m}\\
[(\lambda^{x},m) - \lambda_{i}]W^{i}_{k,m} &=  R^{i}_{k,m} \qquad \textrm{cohomological eqs}
\end{align*}$$
And from the cohomological equations, $\Rightarrow W^{i}_{k,m} = \frac{R^{i}_{k,m}}{(\lambda^{x},m) - \lambda_{i}} \quad k\geq 2$

**Remark:** This is possible if $(\lambda^{x},m) - \lambda_{i} \neq 0$.

###### Def: Primary (external) resonances
The "couples $(m, i)$", $i = d+1, \dots, n$ such that $(\lambda^{x},m) - \lambda_{i} = 0$ are called primary (external) resonances.


##### Equations (components) $i=1, \dots, d$
$$\begin{align*}
(\lambda^{x}, m)W_{k,m}^{i} - \lambda_{i}W^{i}_{k,m} + f^{i}_{k,m}&= R^{i}_{k,m}\\
[(\lambda^{x},m) - \lambda_{i}]W^{i}_{k,m} + f^{i}_{k,m} &=  R^{i}_{k,m} \qquad \textrm{cohomolog equations}\end{align*}$$

Now we can choose:
- (A): **Graph style**: $W^{i}_{k,m}=0$, $f^{i}_{k,m} = R^{i}_{k,m}$
- (B): **Normal form style**: $f^{i}_{k,m}=0$, $W^{i}_{k,m} = \frac{R^{i}_{k,m}}{(\lambda^{x},m) - \lambda_{i}}$

**Remark**: THis is possible if $(\lambda^{x},m) - \lambda_{i} \neq 0$

###### Def: Secondary (internal) resonances
The "couples $(m, i)$", $i = 1, \dots, d$ such that $(\lambda^{x},m) - \lambda_{i} = 0$ are called secondary (internal) resonances.


- In case (A), we obtain:
	$$W(s) = \begin{pmatrix}\vec{s} \\ 0\end{pmatrix} + \sum\limits_{k\geq2}\begin{pmatrix}W^{x}_{k}(s) \\ W^{y}_{k}(s)\end{pmatrix} = \begin{pmatrix}W^{x}(s) \\ W^{y}(s)\end{pmatrix} = \begin{pmatrix}s \\ W^{y}(s)\end{pmatrix}$$ which is a graph (as in $x$ and $f(x)$), and $$f(s)=\begin{pmatrix}\lambda_{1}s_{1} \\ \vdots \\ \lambda_{d}s_{d}\end{pmatrix} + \sum\limits_{k\geq2}f_{k}(s)$$
- In case (b), we obtain:
	$$f(s) = \begin{pmatrix}\lambda_{1}s_{1} \\ \vdots  \\ \lambda_{d}s_{d}\end{pmatrix}$$
	and $$W(s) = \begin{pmatrix}\vec{s} \\ 0\end{pmatrix} + \sum\limits_{k\geq2}\begin{pmatrix}W^{x}_{k}(s) \\ W^{y}_{k}(s)\end{pmatrix} = \begin{pmatrix}W^{x}(s) \\ W^{y}(s)\end{pmatrix}$$
> At each stage, you just have to compute $R$


#### Comments:
###### Comment 1
There are no primary resonances for an unstable or stable invariant manifold.

*Why?*
Let's consider $1\leq i \leq d$, $d+1\leq j \leq n$

If we want to compute a $d$ unstable manifold, this means $Re{(\lambda_{i})>0}$, $Re{(\lambda_{j})<0}$ (case 1):
	$(\lambda^{x},m) - \lambda_{i} = m_{1}\lambda_{1}+\dots + m_{d}\lambda_{d} - \lambda_{j}$
	Take the real part and we have:
	$$m_{1}Re(\lambda_{1}) + \dots + m_{d}Re(\lambda_{d}) - Re(\lambda_{j}) \neq 0$$
	because the first part is always positive ($m$ and $Re(\lambda_{i})$) are always positive and $Re(\lambda_{j})$ will always be negative or zero (since these correspond to the eigenvalues with negative equal part, the ones non-related to the unstable manifold).
	The equivalent for stable manifolds is true.

###### Comment 2
In case of 1D unstable or stable manifolds, there are no secondary resonances: 
	$$(\lambda_{1}, m) - \lambda_{1}=(m-1)\lambda_{1}\neq 0$$ and for $m\geq 2$, so $m-1\leq 0$ and $\lambda_{1}\neq 0$.


> Stable means expansion
> Unstable means compression
> Central means no expansion, no compression.


## Examples
### Example 1 (by hand)
*Assignment*
Consider the pendulum $x'' + \sin{x} = 0$ or equivalently $$\begin{align*}
x_1' &= x_2\\
x_2' &= -\sin{x}
\end{align*}$$
and the equilibrium point $(\pi, 0)$

**Part 1**: Compute, by hand, a parametrization of $\mathfrak{W}^{u}$ (the unstable 1d manifold) up to order 3 (included) following the steps just described using:
	A) Graph style
	B) Normal form style

	![[2.2 Expansion of parametrizations of invariant manifolds (for flows) 2022-11-22 15.13.10.excalidraw]]
We will have $$DG(Z_{0}) = \begin{pmatrix}0 & 1 \\ 1  & 0\end{pmatrix}$$ with eigenvalues $\lambda_{1}= 1$ and $\lambda_{2}= -1$ and $$P=\begin{pmatrix}1 & 1 \\ 1 & -1\end{pmatrix}$$

Remember to do the final step!! $W^{or var}(s) = Z_{0}+ PW(s)$

**Part 2**: Consider the window $[0, 2\pi] \times [-2.5, 2.5]$ and plot the phase portrait and on top the $W^{s}$
![[2.2 Expansion of parametrizations of invariant manifolds (for flows) 2022-11-22 15.20.51.excalidraw]]

### Example 2: The Lorenz manifold
**Goal**: To ocmpute an expansion for the parametrization of the stable manifold of the origin using the normal form style

$$\begin{cases}
x_{1}' &= \sigma(x_{2}-x_{1}) \\
x_{2}' &= \rho x_{1}-x_{2}-x_{1}x_3 \\
x_{3}' &= x_{1}x_{2}-\beta x_{3} \\
\end{cases}$$
with $\sigma=10, \rho=28, \beta= \frac{8}{3}$.

**Eq points**:
$$\begin{align*}
P_{0}=(0, 0, 0)\\
P_{1,2} = (\pm \sqrt{\beta(\rho-1)}, \pm \sqrt{\beta(\rho-1)}, \rho-1)\\
\end{align*}$$
The eigenvalues are $\lambda_{1}=-22.828\dots$, $\lambda_{2}=-2.666\dots$ and $\lambda_{3}=11.828\dots$. This means we have a 1d ustable manifold $\mathfrak{W}^{u}$ and a 2d stable manifold $\mathfrak{W}^{s}$, called the **Lorenz Manifold**.

*Order of the expansion?*
In order to know at a given degree $k$ how good is the expansion, you can check with the invariance condition.

Fix a $k$: $\mathfrak{W}^{s}$ is a 2d manifold.
Consider $s_{\delta,\theta} = (\delta \cos{\theta}, \delta \sin{\theta})$ with $\delta$ fixed and $\theta \in [0, 2\pi)$ (a circle of initial conditions).

Since we are using the normal form style,
$$\begin{cases}
s_{1}' &= \lambda_{1}s_{1}\qquad \Rightarrow \qquad s_{1}(t) = s_{10}e^{\lambda_{1}t} \\
s_{2}' &= \lambda_{2}s_{2}\qquad \Rightarrow \qquad s_{2}(t) = s_{20}e^{\lambda_{2}t} \\
\end{cases}$$
and $\phi_{t}(s_{10}e^{\lambda_{1}t}, s_{20}e^{\lambda_{2}t})$

- Take an $s=s_{0}=s_{\delta, \theta}$ for $\theta$ given. Compute $\phi_t(s)$ for some $t$.
- $W(s) = W(s_{0})$ and compute $\Phi_{t}(W(s))$ for some $t$
- We call $e_{0}(t, s_{\delta, \theta}) = ||W(s(t)) - Z(t)||$
- You compute the error for several $\theta$ and you compute $\epsilon(\delta) = \max_{\theta \in [0, 2\pi]}{e_{0}(t, s_{\delta, \theta})}$

For a given $k$, the smaller $\delta$ is, the smaller the error is. 

Error depends on $t$. Here they take $t=0.3$. The idea is that from $s_{0}$ you go to approx $1000s_0$